extract/main.ml
@@ -1,23 +1,10 @@
+open Regalloc
 open Ssara
-open Gen
-
-let regalloc program fuel =
-  let (programinfo, _) = analyze_program program fuel in  (* Get liveness info *)
-  let interfgraph = get_ig programinfo in                 (* Get interference graph *)
-  let peo = eliminate interfgraph in                      (* Get peo *)
-  let coloring =                                          (* Get coloring *)
-    match get_coloring peo interfgraph with
-    | Some c -> c
-    | None -> failwith "Not enough registers to complete allocation"
-  in
-  let irpreg_program = color_program coloring program in  (* SSA destruction *)
-  ssa_destruct irpreg_program
-;;
 
 let main () =
-  let irvreg_program = Example3.example_block_1 in
-  let irpreg_program = regalloc irvreg_program 10 in
-  gen_irpreg_program irpreg_program
+  let _rv = regalloc_and_run_native Example2.example_block_1 in
+  let _rv = regalloc_and_run_native Example3.example_block_1 in
+  0
 ;;
 
-main ()
+main ();;
