extract/regalloc.ml
@@ -1,0 +1,54 @@
+open Ssara
+open Gen
+
+let fuel = 10;;
+
+let regalloc irvreg_program =
+  let (programinfo, _) = analyze_program irvreg_program fuel in (* Get liveness info *)
+  let interfgraph = get_ig programinfo in                       (* Get interference graph *)
+  let peo = eliminate interfgraph in                            (* Get peo *)
+  let coloring =                                                (* Get coloring *)
+    match get_coloring peo interfgraph with
+    | Some c -> c
+    | None -> failwith "Not enough registers to complete allocation"
+  in
+  let irpreg_program = color_program coloring irvreg_program in (* SSA destruction *)
+  ssa_destruct irpreg_program
+;;
+
+let command_fail cmd =
+  failwith (Printf.sprintf "Failed to execute command: %s\n" cmd)
+;;
+
+let run_native irpreg_program =
+  let asm_filename = "main.asm" in
+  let obj_filename = "main.o" in
+  let bin_filename = "main" in
+
+  (* Generate asm file*)
+  let out = Out_channel.open_text asm_filename in
+  gen_irpreg_program out irpreg_program;
+  Out_channel.close out;
+
+  (* Define commands *)
+  let cmd_asm = Printf.sprintf "nasm -f elf64 -o %s %s" obj_filename asm_filename in
+  let cmd_obj = Printf.sprintf "ld -o %s %s" bin_filename obj_filename in
+  let cmd_bin = Printf.sprintf "./%s" bin_filename in
+
+  (* Assemble asm file *)
+  let rv = Sys.command cmd_asm in
+  if rv <> 0 then command_fail cmd_asm;
+
+  (* Link object file *)
+  let rv = Sys.command cmd_obj in
+  if rv <> 0 then command_fail cmd_obj;
+
+  (* Run binary file and clean compilation files *)
+  let rv = Sys.command cmd_bin in
+  Sys.remove asm_filename; Sys.remove obj_filename; Sys.remove bin_filename;
+  rv
+;;
+
+let regalloc_and_run_native irvreg_program =
+  irvreg_program |> regalloc |> run_native
+;;
