core/Peo.v
@@ -9,20 +9,20 @@ From Ssara.Core Require Import IRVregModule.
 Import IRVreg.
 
 (* Check whether regs are neighbors of r *)
-Definition are_neighbors (g : InterfGraph.dict) (r : reg) (regs : list reg) : bool :=
+Definition are_neighborsb (g : InterfGraph.dict) (r : reg) (regs : list reg) : bool :=
   regs_mem r (InterfGraph.keys g) &&
   conjunction (fun r' => (r =? r') || regs_mem r' (InterfGraph.get g r)) regs
 .
 
 (* Check whether the neighbors of r are a clique *)
-Definition is_simplicial (g : InterfGraph.dict) (r : reg) : bool :=
-  let regs := InterfGraph.get g r in
+Definition is_simplicialb (g : InterfGraph.dict) (r : reg) : bool :=
+  let nbors := InterfGraph.get g r in
   regs_mem r (InterfGraph.keys g) &&
-  conjunction (fun r' => are_neighbors g r' regs) regs
+  conjunction (fun r' => are_neighborsb g r' nbors) nbors
 .
 
 Definition find_next (g : InterfGraph.dict) : option reg :=
-  find (is_simplicial g) (InterfGraph.keys g)
+  find (is_simplicialb g) (InterfGraph.keys g)
 .
 
 Lemma find_next_in :
@@ -50,3 +50,64 @@ Proof.
   apply ig_size_decrease.
   assumption.
 Qed.
+
+(*
+  Proof of correctness of the algorithm that is, the result of the eliminate
+  function is actually a PEO.
+  We start by defining a lemma proving the correctness of a single iteration of
+  the eliminate function, that is proving that `find_next` actually returns a
+  simplicial node.
+*)
+Lemma find_next_simplicial :
+  forall (g : InterfGraph.dict) (r : reg),
+    find_next g = Some r -> is_simplicialb g r = true
+.
+Proof.
+  intros g r. unfold find_next. apply find_some.
+Qed.
+
+(* Now we define a predicate for the simplicial property *)
+Definition is_simplicial (g : InterfGraph.dict) (r : reg) : Prop :=
+  let nbors := InterfGraph.get g r in
+  forall (n n': reg),
+    In n (InterfGraph.keys g) /\ In n' (InterfGraph.keys g) ->
+    In n (InterfGraph.get g n') /\ In n' (InterfGraph.get g n)
+.
+
+(*
+  And the we prove that the `is_simplicialb` function satisfies the
+  `is_simplicial` predicate.
+*)
+(*Lemma is_simplicialb_is_simplicial :
+  forall (g : InterfGraph.dict) (r : reg),
+    is_simplicialb g r = true -> is_simplicial g r
+.
+Proof.
+  intros g r. unfold is_simplicialb.*)
+
+(* Fixpoint split_by (rs : list reg) (r : reg) : list reg :=
+  match rs with
+  | nil => nil
+  | x :: xs => if r =? x then xs else split_by xs r
+  end
+.
+
+Theorem eliminate_result_is_peo :
+  forall (g : InterfGraph.dict) (r : reg),
+    let peo := eliminate g in
+    let after := split_by (InterfGraph.keys g) r
+    In r peo -> after
+.
+
+Definition is_simplicial (g : InterfGraph.dict) (r : reg) : Prop :=
+  let nbors := InterfGraph.get g r in
+  forall (n n': reg),
+    In n nbors /\ In n' nbors
+.
+
+Lemma is_simplicialb_is_simplicial :
+  forall (g : InterfGraph.dict) (r : reg),
+    is_simplicialb g r = true -> is_simplicial g r
+.
+Proof.
+Admitted. *)
